src/arch/x64/Views.fst
@@ -1,0 +1,33 @@
+module Views
+
+open LowStar.BufferView
+open Words_s
+open Types_s
+
+let nat8s_to_nat64 (v1 v2 v3 v4 v5 v6 v7 v8:nat8) : nat64 =
+    v1 + 
+    v2 `op_Multiply` 0x100 + 
+    v3 `op_Multiply` 0x10000 +
+    v4 `op_Multiply` 0x1000000 + 
+    v5 `op_Multiply` 0x100000000 +
+    v6 `op_Multiply` 0x10000000000 +
+    v7 `op_Multiply` 0x1000000000000 +
+    v8 `op_Multiply` 0x100000000000000
+
+let get64 (s:Seq.lseq UInt8.t 8) =
+  UInt64.uint_to_t (
+  nat8s_to_nat64
+    (UInt8.v (Seq.index s 0))
+    (UInt8.v (Seq.index s 1))
+    (UInt8.v (Seq.index s 2))    
+    (UInt8.v (Seq.index s 3))
+    (UInt8.v (Seq.index s 4))
+    (UInt8.v (Seq.index s 5))
+    (UInt8.v (Seq.index s 6))
+    (UInt8.v (Seq.index s 7))    
+  )
+
+assume val put64 (a:UInt64.t) : GTot (Seq.lseq UInt8.t 8)
+assume val inverses64 (u:unit) : Lemma (inverses get64 put64)
+
+let view64 = inverses64 (); View 8 get64 put64
